theories/examples/sort_fg_client.v
@@ -11,16 +11,16 @@ Definition send_all : val :=
     send "c" #cont;; send "c" (lpop "xs");; "go" "c" "xs".
 
 Definition recv_all : val :=
-  rec: "go" "c" :=
-    if: ~recv "c" then lnil #() else
+  rec: "go" "c" "ys" :=
+    if: ~recv "c" then #() else
     let: "x" := recv "c" in
-    let: "l" := "go" "c" in lcons "x" "l";; "l".
+    "go" "c" "ys";; lcons "x" "ys".
 
 Definition sort_client_fg : val := λ: "cmp" "xs",
   let: "c" := start_chan (λ: "c", sort_service_fg "cmp" "c") in
   send_all "c" "xs";;
   send "c" #stop;;
-  recv_all "c".
+  recv_all "c" "xs".
 
 Section sort_fg_client.
   Context `{!heapG Σ, !proto_chanG Σ} (N : namespace).
@@ -29,7 +29,7 @@ Section sort_fg_client.
   Lemma send_all_spec c p xs' l xs :
     {{{ llist I l xs ∗ c ↣ sort_fg_head_protocol I R xs' <++> p @ N }}}
       send_all c #l
-    {{{ RET #(); c ↣ sort_fg_head_protocol I R (xs' ++ xs) <++> p @ N }}}.
+    {{{ RET #(); llist I l [] ∗ c ↣ sort_fg_head_protocol I R (xs' ++ xs) <++> p @ N }}}.
   Proof.
     iIntros (Φ) "[Hl Hc] HΦ".
     iInduction xs as [|x xs] "IH" forall (xs').
@@ -40,40 +40,39 @@ Section sort_fg_client.
     wp_send with "[$HIx]". wp_apply ("IH" with "Hl Hc"). by rewrite -assoc_L.
   Qed.
 
-  Lemma recv_all_spec c p xs ys' :
+  Lemma recv_all_spec c p l xs ys' :
     Sorted R ys' →
-    {{{ c ↣ sort_fg_tail_protocol I R xs ys' <++> p @ N }}}
-      recv_all c
-    {{{ l ys, RET #l;
+    {{{ llist I l [] ∗ c ↣ sort_fg_tail_protocol I R xs ys' <++> p @ N }}}
+      recv_all c #l
+    {{{ ys, RET #();
         ⌜Sorted R (ys' ++ ys)⌝ ∗ ⌜ys' ++ ys ≡ₚ xs⌝ ∗ llist I l ys ∗ c ↣ p @ N
     }}}.
   Proof.
-    iIntros (Hsort Φ) "Hc HΦ".
+    iIntros (Hsort Φ) "[Hl Hc] HΦ".
     iLöb as "IH" forall (xs ys' Φ Hsort).
     wp_lam. wp_branch as %_ | %Hperm; wp_pures.
     - wp_recv (y v) as (Htl) "HIx".
-      wp_apply ("IH" with "[] Hc"); first by auto using Sorted_snoc.
-      iIntros (l ys). rewrite -!assoc_L. iDestruct 1 as (??) "[Hl Hc]".
+      wp_apply ("IH" with "[] Hl Hc"); first by auto using Sorted_snoc.
+      iIntros (ys). rewrite -!assoc_L. iDestruct 1 as (??) "[Hl Hc]".
       wp_apply (lcons_spec with "[$Hl $HIx]"); iIntros "Hl"; wp_pures.
       iApply ("HΦ" with "[$Hl $Hc]"); simpl; eauto.
-    - wp_apply (lnil_spec with "[//]"); iIntros (l) "Hl".
-      iApply ("HΦ" $! _ []); rewrite /= right_id_L; by iFrame.
+    - iApply ("HΦ" $! []); rewrite /= right_id_L; by iFrame.
   Qed.
 
   Lemma sort_client_fg_spec cmp l xs :
     cmp_spec I R cmp -∗
     {{{ llist I l xs }}}
       sort_client_fg cmp #l
-    {{{ k ys, RET #k; ⌜Sorted R ys⌝ ∗ ⌜ys ≡ₚ xs⌝ ∗ llist I k ys }}}.
+    {{{ ys, RET #(); ⌜Sorted R ys⌝ ∗ ⌜ys ≡ₚ xs⌝ ∗ llist I l ys }}}.
   Proof.
     iIntros "#Hcmp !>" (Φ) "Hl HΦ". wp_lam.
     wp_apply (start_chan_proto_spec N (sort_fg_protocol I R <++> END)%proto);
       iIntros (c) "Hc".
     { wp_apply (sort_service_fg_spec N with "Hcmp Hc"); auto. }
-    wp_apply (send_all_spec with "[$Hl $Hc]"); iIntros "Hc".
+    wp_apply (send_all_spec with "[$Hl $Hc]"); iIntros "[Hl Hc]".
     wp_select.
-    wp_apply (recv_all_spec with "Hc"); auto.
-    iIntros (k ys) "/=". iDestruct 1 as (??) "[Hk _]".
+    wp_apply (recv_all_spec with "[$Hl $Hc]"); auto.
+    iIntros (ys) "/=". iDestruct 1 as (??) "[Hk _]".
     iApply "HΦ"; auto with iFrame.
   Qed.
 End sort_fg_client.
